Started some of the SplayHeap proofs

examples/miniML/okasaki-examples/SplayHeapScript.sml
@@ -1,4 +1,4 @@
-open bossLib Theory Parse boolTheory pairTheory Defn Tactic boolLib
+open bossLib Theory Parse boolTheory pairTheory Defn Tactic boolLib bagTheory
 open lcsymtacs;
 
 val fs = full_simp_tac (srw_ss ())
@@ -15,6 +15,17 @@ val _ = new_theory "SplayHeap"
 val _ = Hol_datatype `
 heaps = Empty | Node of heaps => 'a => heaps`;
 
+val splay_heap_to_bag_def = Define `
+(splay_heap_to_bag Empty = {||}) ∧
+(splay_heap_to_bag (Node h1 x h2) =
+  BAG_INSERT x (BAG_UNION (splay_heap_to_bag h1) (splay_heap_to_bag h2)))`;
+
+val splay_heap_ok_def = Define `
+(splay_heap_ok leq Empty = T) ∧
+(splay_heap_ok leq (Node h1 x h2) = 
+  (!y. BAG_IN y (splay_heap_to_bag h1) ⇒ leq y x) ∧
+  (!y. BAG_IN y (splay_heap_to_bag h2) ⇒ ¬leq y x))`;
+
 val _ = Define `
 empty = Empty`;
 
@@ -23,85 +34,129 @@ val _ = Define `
 (is_empty _ = F)`;
 
 val partition_def = Define `
-(partition element_leq pivot Empty = (Empty, Empty)) ∧
-(partition element_leq pivot (Node a x b) =
-  if element_leq x pivot then
+(partition leq pivot Empty = (Empty, Empty)) ∧
+(partition leq pivot (Node a x b) =
+  if leq x pivot then
     (case b of
         Empty => (Node a x b, Empty)
       | Node b1 y b2 =>
-          if element_leq y pivot then
-            let (small, big) = partition element_leq pivot b2 in
+          if leq y pivot then
+            let (small, big) = partition leq pivot b2 in
               (Node (Node a x b1) y small, big)
           else
-            let (small, big) = partition element_leq pivot b1 in
+            let (small, big) = partition leq pivot b1 in
               (Node a x small, Node big y b2))
   else
     (case a of
         Empty => (Empty, Node a x b)
       | Node a1 y a2 =>
-          if element_leq y pivot then
-            let (small, big) = partition element_leq pivot a2 in
+          if leq y pivot then
+            let (small, big) = partition leq pivot a2 in
               (Node a1 y small, Node big x b)
           else
-            let (small, big) = partition element_leq pivot a1 in
+            let (small, big) = partition leq pivot a1 in
               (small, Node big y (Node a2 x b))))`;
 
 val partition_ind = fetch "-" "partition_ind" 
 val heaps_size_def = fetch "-" "heaps_size_def" 
 
-val partition_smaller = Q.prove (
-`!element_leq p h1 h2 h3.
-  ((h2,h3) = partition element_leq p h1)
+val partition_thm = Q.prove (
+`!leq p h1 h2 h3.
+  ((h2,h3) = partition leq p h1)
   ⇒
+  (splay_heap_to_bag h1 = 
+   BAG_UNION (splay_heap_to_bag h2) (splay_heap_to_bag h3)) ∧
   heaps_size f h2 ≤ heaps_size f h1 ∧
   heaps_size f h3 ≤ heaps_size f h1`,
 recInduct partition_ind >>
-rw [heaps_size_def, partition_def] >>
+rw [heaps_size_def, partition_def, splay_heap_to_bag_def] >>
+full_case_tac >>
+fs [] >>
+rw [heaps_size_def, splay_heap_to_bag_def] >>
 full_case_tac >>
 fs [] >>
 rw [heaps_size_def] >>
-full_case_tac >>
-fs [] >>
-rw [heaps_size_def] >|
-[cases_on `partition element_leq pivot h0`,
- cases_on `partition element_leq pivot h`,
- cases_on `partition element_leq pivot h0`,
- cases_on `partition element_leq pivot h`,
- cases_on `partition element_leq pivot h0`,
- cases_on `partition element_leq pivot h`,
- cases_on `partition element_leq pivot h0`,
- cases_on `partition element_leq pivot h`] >>
+cases_on `partition leq pivot h0` >>
+cases_on `partition leq pivot h` >>
 fs [LET_THM] >>
-rw [heaps_size_def] >>
-decide_tac);
+rw [heaps_size_def, splay_heap_to_bag_def, BAG_UNION_INSERT] >|
+[metis_tac [ASSOC_BAG_UNION, COMM_BAG_UNION, BAG_INSERT_commutes],
+ metis_tac [ASSOC_BAG_UNION, COMM_BAG_UNION, BAG_INSERT_commutes],
+ decide_tac,
+ decide_tac,
+ decide_tac,
+ decide_tac,
+ metis_tac [ASSOC_BAG_UNION, COMM_BAG_UNION, BAG_INSERT_commutes],
+ metis_tac [ASSOC_BAG_UNION, COMM_BAG_UNION, BAG_INSERT_commutes],
+ decide_tac,
+ decide_tac,
+ decide_tac,
+ decide_tac]);
 
-val _ = Define `
-(insert element_leq x t = 
-  let (a, b) = partition element_leq x t in 
-    Node a x b)`;
+val insert_def = Define `
+insert leq x t = 
+  let (a, b) = partition leq x t in 
+    Node a x b`;
 
 val merge_def = tDefine "merge" `
-(merge element_leq Empty h2 = h2) ∧
-(merge element_leq (Node a x b) h2 =
-  let (ta, tb) = partition element_leq x h2 in
-    Node (merge element_leq ta a) x (merge element_leq tb b))`
+(merge leq Empty h2 = h2) ∧
+(merge leq (Node a x b) h2 =
+  let (ta, tb) = partition leq x h2 in
+    Node (merge leq ta a) x (merge leq tb b))`
 (WF_REL_TAC `measure (\(x,y,z). 
                         heaps_size (\_.1) y + 
                         heaps_size (\_.1) z)` >>
  rw [] >>
- imp_res_tac partition_smaller >>
+ imp_res_tac partition_thm >>
  pop_assum (MP_TAC o Q.SPEC `(λ_.1)`) >>
  pop_assum (MP_TAC o Q.SPEC `(λ_.1)`) >>
- full_simp_tac (srw_ss() ++ ARITH_ss) [partition_smaller]); 
+ full_simp_tac (srw_ss() ++ ARITH_ss) [partition_thm]); 
 
-val find_min_defn = Define `
+val merge_ind = fetch "-" "merge_ind"
+
+val find_min_def = Define `
 (find_min (Node Empty x b) = x) ∧
 (find_min (Node a x b) = find_min a)`;
 
-val delete_min_defn = Hol_defn "delete_min" `
+val find_min_ind = fetch "-" "find_min_ind"
+
+val delete_min_defn = Define `
 (delete_min (Node Empty x b) = b) ∧
 (delete_min (Node (Node Empty x b) y c) = Node b y c) ∧
 (delete_min (Node (Node a x b) y c) = Node (delete_min a) x (Node b y c))`;
+
+val insert_thm = Q.store_thm ("insert_thm",
+`!h leq x. 
+  splay_heap_to_bag (insert leq x h) = 
+  BAG_INSERT x (splay_heap_to_bag h)`,
+induct_on `h` >>
+rw [splay_heap_to_bag_def, insert_def] >>
+rw [splay_heap_to_bag_def] >>
+fs [insert_def] >>
+imp_res_tac (GSYM partition_thm) >>
+fs [splay_heap_to_bag_def]);
+
+val merge_thm = Q.store_thm ("merge_thm",
+`!leq h1 h2.
+  (splay_heap_to_bag (merge leq h1 h2) =
+    BAG_UNION (splay_heap_to_bag h1) (splay_heap_to_bag h2))`,
+recInduct merge_ind >>
+rw [merge_def, splay_heap_to_bag_def] >>
+cases_on `partition leq x h2` >>
+fs [] >>
+imp_res_tac (GSYM partition_thm) >>
+rw [splay_heap_to_bag_def, BAG_UNION_INSERT] >>
+metis_tac [ASSOC_BAG_UNION, COMM_BAG_UNION, BAG_INSERT_commutes]);
+
+(*
+val find_min_thm = Q.prove (
+`!h x leq. (h ≠ Empty) ∧ splay_heap_ok leq h ⇒
+  ((find_min h = x) = 
+   (BAG_IN x (splay_heap_to_bag h) ∧
+    (!y. BAG_IN y (splay_heap_to_bag h) ⇒ leq x y)))`,
+recInduct find_min_ind >>
+rw [splay_heap_to_bag_def, splay_heap_ok_def, find_min_def] >-
+*)
 
 val _ = export_theory()
 
